Regenerate the tests

tests/lean/External/Types.lean
@@ -9,10 +9,4 @@ set_option linter.unusedVariables false
 
 namespace external
 
-/- Trait declaration: [core::marker::Copy]
-   Source: '/rustc/library/core/src/marker.rs', lines 416:0-416:21
-   Name pattern: core::marker::Copy -/
-structure core.marker.Copy (Self : Type) where
-  cloneCloneInst : core.clone.Clone Self
-
 end external
