tests/fstar/misc/External.Funs.fst
@@ -7,13 +7,6 @@ include External.FunsExternal
 
 #set-options "--z3rlimit 50 --fuel 1 --ifuel 1"
 
-(** Trait implementation: [core::marker::{core::marker::Copy for u32}#40]
-    Source: '/rustc/library/core/src/marker.rs', lines 48:25-48:62
-    Name pattern: core::marker::Copy<u32> *)
-let core_marker_CopyU32 : core_marker_Copy_t u32 = {
-  cloneCloneInst = core_clone_CloneU32;
-}
-
 (** [external::use_get]:
     Source: 'tests/src/external.rs', lines 9:0-11:1 *)
 let use_get (rc : core_cell_Cell_t u32) (st : state) : result (state & u32) =
